Huge refactoring of the MESI simulation proof, in order for MOSI to use common proofs.

src/Common.v
@@ -245,25 +245,6 @@ Module PropMonadNotations.
   Open Scope monad_scope.
 End PropMonadNotations.
 
-Fixpoint caseDec {A B} (dec: forall a1 a2: A, {a1 = a2} + {a1 <> a2})
-         (a: A) (def: B) (cs: list (A * B)) :=
-  match cs with
-  | List.nil => def
-  | List.cons (ca, cp) cs' =>
-    if dec a ca then cp else caseDec dec a def cs'
-  end.
-
-Module CaseNotations.
-  Notation "x : t" := (x, t) (at level 90, only parsing): cases_scope.
-  Notation "|! xt" := (List.cons xt List.nil) (at level 95, only parsing): cases_scope.
-  Notation "| xt1 | xt2 | .. | xtn" :=
-    (List.cons xt1 (List.cons xt2 .. (List.cons xtn List.nil) ..))
-      (at level 95, only parsing): cases_scope.
-  Delimit Scope cases_scope with cases.
-  Notation "'match' 'case' X 'on' DEC 'default' DEF 'with' CS 'end'" :=
-    (caseDec DEC X DEF CS%cases) (only parsing).
-End CaseNotations.
-
 Inductive PHide: Prop -> Prop :=
 | PHideIntro: forall P:Prop, P -> PHide P.
 
