src/Ex/Mesi/MesiInv.v
@@ -4,7 +4,8 @@ Require Import Invariant TrsInv Simulation Serial SerialFacts.
 Require Import RqRsLang RqRsCorrect.
 
 Require Import Ex.Spec Ex.SpecInds Ex.Template.
-Require Import Ex.Mesi Ex.Mesi.Mesi Ex.Mesi.MesiTopo Ex.Mesi.MesiInvB.
+Require Import Ex.Mesi Ex.Mesi.Mesi Ex.Mesi.MesiTopo.
+Require Import Ex.InvTemplate Ex.Mesi.MesiInvB.
 
 Set Implicit Arguments.
 
@@ -17,20 +18,20 @@ Local Open Scope fmap.
 
 Existing Instance Mesi.ImplOStateIfc.
 
-(** Common Invariants that might be shared with the MOSI case study *)
-
-Definition MsgExistsSig (sig: MSig) (msgs: MessagePool Msg) :=
-  exists idm, InMPI msgs idm /\ sigOf idm = sig.
-
-Definition MsgP (spl: list (MSig * (Id Msg -> Prop))) (idm: Id Msg) :=
-  caseDec sig_dec (sigOf idm) True
-          (map (fun sp => (fst sp, snd sp idm)) spl).
-
-Definition MsgsP (spl: list (MSig * (Id Msg -> Prop))) (msgs: MessagePool Msg) :=
-  forall idm, InMPI msgs idm -> MsgP spl idm.
-
-Definition MsgsNotExist (sigs: list MSig) (msgs: MessagePool Msg) :=
-  MsgsP (map (fun sig => (sig, fun _ => False)) sigs) msgs.
+Lemma mesi_RsDownConflicts:
+  forall tr (Htr: tr <> Node nil),
+    InvReachable (impl Htr) step_m (MsgConflictsInv tr 0).
+Proof.
+  intros.
+  apply tree2Topo_MsgConflicts_inv_ok; auto.
+  simpl; unfold mem, li, l1.
+  rewrite map_app.
+  do 2 rewrite map_trans.
+  do 2 rewrite map_id.
+  rewrite app_comm_cons.
+  rewrite <-c_li_indices_head_rootOf by assumption.
+  apply SubList_refl.
+Qed.
 
 Section CoherenceUnit.
   Variables (oidx: IdxT)
@@ -129,179 +130,6 @@ Section CoherenceUnit.
 
 End CoherenceUnit.
 
-Section MsgConflicts.
-
-  Definition RsDownConflicts (oidx: IdxT) (orq: ORq Msg) (msgs: MessagePool Msg) :=
-    forall rsDown,
-      fst (sigOf rsDown) = downTo oidx ->
-      fst (snd (sigOf rsDown)) = MRs ->
-      InMPI msgs rsDown ->
-      (orq@[upRq] <> None) /\
-      (forall rqUp,
-          fst (sigOf rqUp) = rqUpFrom oidx ->
-          InMPI msgs rqUp -> False) /\
-      (forall rrsDown,
-          fst (sigOf rrsDown) = downTo oidx ->
-          fst (snd (sigOf rrsDown)) = MRs ->
-          valOf rsDown <> valOf rrsDown ->
-          InMPI msgs rrsDown -> False) /\
-      (forall rqDown,
-          fst (sigOf rqDown) = downTo oidx ->
-          fst (snd (sigOf rqDown)) = MRq ->
-          FirstMPI msgs rqDown -> False) /\
-      (forall rsUp,
-          fst (sigOf rsUp) = rsUpFrom oidx ->
-          InMPI msgs rsUp -> False).
-
-  Definition RqUpConflicts (oidx: IdxT) (orq: ORq Msg) (msgs: MessagePool Msg) :=
-    forall rqUp,
-      fst (sigOf rqUp) = rqUpFrom oidx ->
-      InMPI msgs rqUp ->
-      (orq@[upRq] <> None) /\
-      (forall rrqUp,
-          fst (sigOf rrqUp) = rqUpFrom oidx ->
-          valOf rqUp <> valOf rrqUp ->
-          InMPI msgs rrqUp -> False) /\
-      (forall rsDown,
-          fst (sigOf rsDown) = downTo oidx ->
-          fst (snd (sigOf rsDown)) = MRs ->
-          InMPI msgs rsDown -> False).
-
-  Variable (tr: tree) (bidx: IdxT).
-  Hypothesis (Htr: tr <> Node nil).
-  Let topo := fst (tree2Topo tr bidx).
-  Let cifc := snd (tree2Topo tr bidx).
-
-  Context `{OStateIfc}.
-  Variable (sys: System).
-  
-  Hypotheses (Hiorqs: GoodORqsInit (initsOf sys))
-             (Hrrs: RqRsSys topo sys)
-             (Hoinds: SubList (c_li_indices cifc ++ c_l1_indices cifc)
-                              (map (@obj_idx _) (sys_objs sys))).
-
-  Definition MsgConflictsInv (st: MState) :=
-    forall oidx orq,
-      In oidx (c_li_indices cifc ++ c_l1_indices cifc) ->
-      (bst_orqs st)@[oidx] = Some orq ->
-      RsDownConflicts oidx orq (bst_msgs st) /\
-      RqUpConflicts oidx orq (bst_msgs st).
-
-  Lemma tree2Topo_MsgConflicts_inv_ok:
-    InvReachable sys step_m MsgConflictsInv.
-  Proof.
-    unfold InvReachable, MsgConflictsInv; intros.
-
-    unfold cifc in H1.
-    rewrite c_li_indices_head_rootOf in H1 by assumption.
-    inv H1.
-
-    1: { (* the root case *)
-      (** TODO: need to prove an invariant about the root (main memory):
-       * no messages exist in any channel of the root, i.e., the RqUp, RsUp,
-       * and Down queues are all empty for the root.
-       *)
-      admit.
-    }
-
-    (* non-root cases *)
-    assert (exists pidx,
-               In pidx (c_li_indices cifc) /\
-               parentIdxOf topo oidx = Some pidx).
-    { apply in_app_or in H3; destruct H3.
-      { apply c_li_indices_tail_has_parent; assumption. }
-      { apply c_l1_indices_has_parent; assumption. }
-    }
-    destruct H1 as [pidx [? ?]].
-
-    pose proof (tree2Topo_TreeTopo tr bidx).
-    destruct H5; dest.
-    specialize (H5 _ _ H4); dest.
-
-    assert (exists obj, In obj (sys_objs sys) /\ obj_idx obj = oidx).
-    { apply in_app_or in H3; destruct H3.
-      { apply tl_In in H3.
-        apply SubList_app_4 in Hoinds; apply Hoinds in H3.
-        apply in_map_iff in H3; destruct H3 as [obj [? ?]]; subst.
-        exists obj; auto.
-      }
-      { apply SubList_app_5 in Hoinds; apply Hoinds in H3.
-        apply in_map_iff in H3; destruct H3 as [obj [? ?]]; subst.
-        exists obj; auto.
-      }
-    }
-    destruct H10 as [obj [? ?]]; subst.
-
-    assert (exists pobj, In pobj (sys_objs sys) /\ obj_idx pobj = pidx).
-    { apply SubList_app_4 in Hoinds; apply Hoinds in H1.
-      apply in_map_iff in H1; destruct H1 as [pobj [? ?]]; subst.
-      exists pobj; auto.
-    }
-    destruct H11 as [pobj [? ?]]; subst.
-
-    split; red; intros; repeat ssplit; intros.
-    - intro Hx.
-      eapply upLocked_rsDown_in_false
-        with (obj0:= obj) (down:= downTo (obj_idx obj))
-             (rsdm:= valOf rsDown); eauto.
-      unfold sigOf in H12; simpl in H12; red in H14; rewrite H12 in H14; assumption.
-    - eapply rqUp_in_rsDown_in_false
-        with (obj0:= obj) (rqUp0:= rqUpFrom (obj_idx obj)) (rqum:= valOf rqUp)
-             (down:= downTo (obj_idx obj)) (rsdm:= valOf rsDown); eauto.
-      + unfold sigOf in H15; simpl in H15; red in H16; rewrite H15 in H16; assumption.
-      + unfold sigOf in H12; simpl in H12; red in H14; rewrite H12 in H14; assumption.
-    - eapply rsDown_in_rsDown_in_false
-        with (obj0:= obj) (down:= downTo (obj_idx obj))
-             (rsdm1:= valOf rsDown) (rsdm2:= valOf rrsDown); eauto.
-      + unfold sigOf in H12; simpl in H12; red in H14; rewrite H12 in H14; assumption.
-      + unfold sigOf in H15; simpl in H15; red in H18; rewrite H15 in H18; assumption.
-    - eapply rsDown_in_rqDown_first_false
-        with (cobj:= obj) (pobj0:= pobj) (down:= downTo (obj_idx obj))
-             (rsdm:= valOf rsDown) (rqdm:= valOf rqDown); eauto.
-      + unfold sigOf in H12; simpl in H12; red in H14; rewrite H12 in H14; assumption.
-      + unfold sigOf in H15; simpl in H15; red in H17; rewrite H15 in H17; assumption.
-    - eapply rsDown_in_rsUp_in_false
-        with (cobj:= obj) (pobj0:= pobj) (rsUp0:= rsUpFrom (obj_idx obj))
-             (down:= downTo (obj_idx obj))
-             (rsdm:= valOf rsDown) (rsum:= valOf rsUp); eauto.
-      + unfold sigOf in H12; simpl in H12; red in H14; rewrite H12 in H14; assumption.
-      + unfold sigOf in H15; simpl in H15; red in H16; rewrite H15 in H16; assumption.
-    - intro Hx.
-      eapply upLocked_rqUp_in_false
-        with (obj0:= obj) (rqUp0:= rqUpFrom (obj_idx obj))
-             (rqum:= valOf rqUp); eauto.
-      unfold sigOf in H12; simpl in H12; red in H13; rewrite H12 in H13; assumption.
-    - eapply rqUp_in_rqUp_in_false
-        with (obj0:= obj) (rqUp0:= rqUpFrom (obj_idx obj))
-             (rqum1:= valOf rqUp) (rqum2:= valOf rrqUp); eauto.
-      + unfold sigOf in H12; simpl in H12; red in H13; rewrite H12 in H13; assumption.
-      + unfold sigOf in H14; simpl in H14; red in H16; rewrite H14 in H16; assumption.
-    - eapply rqUp_in_rsDown_in_false
-        with (obj0:= obj) (rqUp0:= rqUpFrom (obj_idx obj)) (rqum:= valOf rqUp)
-             (down:= downTo (obj_idx obj)) (rsdm:= valOf rsDown); eauto.
-      + unfold sigOf in H12; simpl in H12; red in H13; rewrite H12 in H13; assumption.
-      + unfold sigOf in H14; simpl in H14; red in H16; rewrite H14 in H16; assumption.
-  Admitted.
-
-End MsgConflicts.
-
-Lemma mesi_RsDownConflicts:
-  forall tr (Htr: tr <> Node nil),
-    InvReachable (impl Htr) step_m (MsgConflictsInv tr 0).
-Proof.
-  intros.
-  apply tree2Topo_MsgConflicts_inv_ok; auto.
-  simpl; unfold mem, li, l1.
-  rewrite map_app.
-  do 2 rewrite map_trans.
-  do 2 rewrite map_id.
-  rewrite app_comm_cons.
-  rewrite <-c_li_indices_head_rootOf by assumption.
-  apply SubList_refl.
-Qed.
-
-(** End of the common invariants -- *)
-
 Definition InvObjExcl0 (oidx: IdxT) (ost: OState) (msgs: MessagePool Msg) :=
   ObjExcl0 oidx ost msgs -> NoCohMsgs oidx msgs.
 
@@ -350,261 +178,7 @@ Definition InvForSim (topo: DTree) (st: MState): Prop :=
   InvWB st /\ InvWBChild topo st /\ InvNonWB topo st /\
   MesiFootprintsInv topo st.
 
-Lemma mesi_InvForSim_init:
-  forall tr (Htr: tr <> Node nil),
-    InvForSim (fst (tree2Topo tr 0)) (initsOf (impl Htr)).
-Proof.
-Admitted.
-
-Lemma mesi_InvForSim_ok:
-  forall tr (Htr: tr <> Node nil),
-    InvStep (impl Htr) step_m (InvForSim (fst (tree2Topo tr 0))).
-Proof.
-Admitted.
-
-Lemma caseDec_head_eq:
-  forall {A B} (eq_dec: forall a1 a2: A, {a1 = a2} + {a1 <> a2})
-         k (df: B) hd tl,
-    k = fst hd ->
-    caseDec eq_dec k df (hd :: tl) = snd hd.
-Proof.
-  intros; subst.
-  destruct hd as [hk hv]; simpl.
-  find_if_inside; [reflexivity|exfalso; auto].
-Qed.
-
-Lemma caseDec_head_neq:
-  forall {A B} (eq_dec: forall a1 a2: A, {a1 = a2} + {a1 <> a2})
-         k (df: B) hd tl,
-    k <> fst hd ->
-    caseDec eq_dec k df (hd :: tl) = caseDec eq_dec k df tl.
-Proof.
-  intros; subst.
-  destruct hd as [hk hv]; simpl.
-  find_if_inside; [exfalso; auto|reflexivity].
-Qed.
-
-Ltac disc_caseDec Hcd :=
-  repeat
-    (first [rewrite caseDec_head_eq in Hcd by reflexivity
-           |rewrite caseDec_head_neq in Hcd by discriminate]);
-  simpl in Hcd.
-
-Ltac solve_caseDec :=
-  repeat
-    (first [rewrite caseDec_head_eq by reflexivity
-           |rewrite caseDec_head_neq by discriminate]);
-  simpl.
-
 Section Facts.
-
-  Lemma MsgsP_enqMP:
-    forall spl msgs,
-      MsgsP spl msgs ->
-      forall midx msg,
-        MsgP spl (midx, msg) ->
-        MsgsP spl (enqMP midx msg msgs).
-  Proof.
-    unfold MsgsP, MsgP; intros.
-    apply InMP_enqMP_or in H1; destruct H1; auto.
-    destruct idm as [midx' msg']; simpl in *; dest; subst.
-    assumption.
-  Qed.
-
-  Lemma MsgsP_other_midx_enqMP:
-    forall spl msgs,
-      MsgsP spl msgs ->
-      forall midx msg,
-        ~ In midx (map (fun sp => fst (fst sp)) spl) ->
-        MsgsP spl (enqMP midx msg msgs).
-  Proof.
-    unfold MsgsP, MsgP; intros.
-    apply InMP_enqMP_or in H1; destruct H1; auto.
-    destruct idm as [midx' msg']; simpl in *; dest; subst.
-    destruct msg as [mid mty mval].
-    unfold sigOf; simpl.
-    clear -H0.
-    induction spl; [simpl; auto|].
-    unfold map; rewrite caseDec_head_neq.
-    - apply IHspl.
-      intro Hx; elim H0; right; assumption.
-    - simpl; intro Hx.
-      elim H0; left.
-      unfold MSig in *; rewrite <-Hx; reflexivity.
-  Qed.
-
-  Lemma MsgsP_other_midx_enqMsgs:
-    forall spl msgs,
-      MsgsP spl msgs ->
-      forall eins,
-        DisjList (idsOf eins) (map (fun sp => fst (fst sp)) spl) ->
-        MsgsP spl (enqMsgs eins msgs).
-  Proof.
-    intros.
-    generalize dependent msgs.
-    induction eins as [|ein eins]; simpl; intros; [assumption|].
-    destruct ein as [midx msg]; simpl in *.
-    apply DisjList_cons in H0; dest.
-    eapply IHeins; eauto.
-    apply MsgsP_other_midx_enqMP; auto.
-  Qed.
-
-  Lemma MsgsP_other_msg_id_enqMP:
-    forall spl msgs,
-      MsgsP spl msgs ->
-      forall midx msg,
-        ~ In (msg_id msg) (map (fun sp => snd (snd (fst sp))) spl) ->
-        MsgsP spl (enqMP midx msg msgs).
-  Proof.
-    unfold MsgsP, MsgP; intros.
-    apply InMP_enqMP_or in H1; destruct H1; auto.
-    destruct idm as [midx' msg']; simpl in *; dest; subst.
-    destruct msg as [mid mty mval]; simpl in H0.
-    unfold sigOf; simpl.
-    clear -H0.
-    induction spl; [simpl; auto|].
-    unfold map; rewrite caseDec_head_neq.
-    - apply IHspl.
-      intro Hx; elim H0; right; assumption.
-    - simpl; intro Hx.
-      elim H0; left.
-      unfold MSig in *; rewrite <-Hx; reflexivity.
-  Qed.
-
-  Lemma MsgsP_other_msg_id_enqMsgs:
-    forall spl msgs,
-      MsgsP spl msgs ->
-      forall eins,
-        DisjList (map (fun idm => msg_id (valOf idm)) eins)
-                 (map (fun sp => snd (snd (fst sp))) spl) ->
-        MsgsP spl (enqMsgs eins msgs).
-  Proof.
-    intros.
-    generalize dependent msgs.
-    induction eins as [|ein eins]; simpl; intros; [assumption|].
-    destruct ein as [midx msg]; simpl in *.
-    apply DisjList_cons in H0; dest.
-    eapply IHeins; eauto.
-    apply MsgsP_other_msg_id_enqMP; auto.
-  Qed.
-
-  Lemma MsgsP_enqMP_inv:
-    forall spl msgs midx msg,
-      MsgsP spl (enqMP midx msg msgs) ->
-      MsgsP spl msgs.
-  Proof.
-    unfold MsgsP; intros.
-    apply H.
-    apply InMP_or_enqMP; auto.
-  Qed.
-
-  Lemma MsgsP_enqMsgs_inv:
-    forall spl msgs eins,
-      MsgsP spl (enqMsgs eins msgs) ->
-      MsgsP spl msgs.
-  Proof.
-    unfold MsgsP; intros.
-    apply H.
-    apply InMP_or_enqMsgs; auto.
-  Qed.
-
-  Lemma MsgsP_deqMP:
-    forall spl msgs,
-      MsgsP spl msgs ->
-      forall midx,
-        MsgsP spl (deqMP midx msgs).
-  Proof.
-    unfold MsgsP; intros.
-    apply InMP_deqMP in H0; auto.
-  Qed.
-
-  Lemma MsgsP_deqMsgs:
-    forall spl msgs,
-      MsgsP spl msgs ->
-      forall minds,
-        MsgsP spl (deqMsgs minds msgs).
-  Proof.
-    unfold MsgsP; intros.
-    apply InMP_deqMsgs in H0; auto.
-  Qed.
-
-  Lemma MsgsP_other_midx_deqMP_inv:
-    forall spl msgs midx,
-      MsgsP spl (deqMP midx msgs) ->
-      ~ In midx (map (fun sp => fst (fst sp)) spl) ->
-      MsgsP spl msgs.
-  Proof.
-    unfold MsgsP, MsgP; intros.
-    destruct (idx_dec midx (idOf idm)); subst;
-      [|apply H; apply deqMP_InMP_midx; auto].
-
-    clear -H0.
-    induction spl; [simpl; auto|].
-    unfold map; rewrite caseDec_head_neq.
-    - apply IHspl.
-      intro Hx; elim H0; right; assumption.
-    - simpl; intro Hx.
-      elim H0; left.
-      unfold MSig in *; rewrite <-Hx; reflexivity.
-  Qed.
-
-  Lemma MsgsP_other_midx_deqMsgs_inv:
-    forall spl minds msgs,
-      MsgsP spl (deqMsgs minds msgs) ->
-      DisjList minds (map (fun sp => fst (fst sp)) spl) ->
-      MsgsP spl msgs.
-  Proof.
-    intros.
-    generalize dependent msgs.
-    induction minds as [|mind minds]; simpl; intros; [assumption|].
-    apply DisjList_cons in H0; dest.
-    eapply MsgsP_other_midx_deqMP_inv.
-    - eapply IHminds; eauto.
-    - assumption.
-  Qed.
-
-  Lemma MsgsP_other_msg_id_deqMP_inv:
-    forall spl msgs midx msg,
-      MsgsP spl (deqMP midx msgs) ->
-      FirstMP msgs midx msg ->
-      ~ In (msg_id msg) (map (fun sp => snd (snd (fst sp))) spl) ->
-      MsgsP spl msgs.
-  Proof.
-    unfold MsgsP, MsgP; intros.
-    destruct (idx_dec midx (idOf idm)); subst;
-      [|apply H; apply deqMP_InMP_midx; auto].
-
-    destruct (msg_dec msg (valOf idm)); subst;
-      [|apply H; eapply deqMP_InMP; eauto; congruence].
-
-    clear -H1.
-    induction spl; [simpl; auto|].
-    unfold map; rewrite caseDec_head_neq.
-    - apply IHspl.
-      intro Hx; elim H1; right; assumption.
-    - simpl; intro Hx.
-      elim H1; left.
-      unfold MSig in *; rewrite <-Hx; reflexivity.
-  Qed.
-
-  Lemma MsgsP_other_msg_id_deqMsgs_inv:
-    forall spl rmsgs msgs,
-      MsgsP spl (deqMsgs (idsOf rmsgs) msgs) ->
-      NoDup (idsOf rmsgs) ->
-      Forall (FirstMPI msgs) rmsgs ->
-      DisjList (map (fun idm => msg_id (valOf idm)) rmsgs)
-               (map (fun sp => snd (snd (fst sp))) spl) ->
-      MsgsP spl msgs.
-  Proof.
-    intros.
-    generalize dependent msgs.
-    induction rmsgs as [|rmsg rmsgs]; simpl; intros; [assumption|].
-    inv H0; inv H1.
-    apply DisjList_cons in H2; dest.
-    eapply MsgsP_other_msg_id_deqMP_inv; eauto.
-    eapply IHrmsgs; eauto.
-    apply FirstMPI_Forall_deqMP; auto.
-  Qed.
 
   Lemma InvExcl_excl_invalid:
     forall st (He: InvExcl st) msgs eidx eost,
@@ -645,6 +219,256 @@ Section Facts.
   
 End Facts.
 
-Hint Unfold MsgsNotExist NoRsI ImplOStateMESI: RuleConds.
+(** The invariants proof starts here -- *)
+
+Lemma mesi_InvForSim_init:
+  forall tr (Htr: tr <> Node nil),
+    InvForSim (fst (tree2Topo tr 0)) (initsOf (impl Htr)).
+Proof.
+Admitted.
+
+Lemma mesi_InvForSim_ok:
+  forall tr (Htr: tr <> Node nil),
+    InvStep (impl Htr) step_m (InvForSim (fst (tree2Topo tr 0))).
+Proof.
+Admitted.
+
+Ltac solve_NoRsI_base :=
+  repeat
+    match goal with
+    | |- NoRsI _ _ => do 3 red; intros
+    | |- MsgP _ _ =>
+      red; unfold map, caseDec, fst;
+      repeat (find_if_inside; [simpl|auto])
+    | [H: sigOf ?idm = _ |- _] =>
+      let midx := fresh "midx" in
+      let msg := fresh "msg" in
+      destruct idm as [midx msg]; inv H
+    end.
+
+Ltac solve_NoRsI_by_no_locks oidx :=
+  repeat
+    match goal with
+    | [Hmcfi: MsgConflictsInv _ _ {| bst_orqs:= ?orqs |},
+              Hin: In oidx (c_l1_indices _),
+                   Horq: ?orqs@[oidx] = Some _ |- _] =>
+      specialize (Hmcfi oidx _ (in_or_app _ _ _ (or_intror Hin)) Horq);
+      simpl in Hmcfi; destruct Hmcfi
+    | [Hmcfi: MsgConflictsInv _ _ {| bst_orqs:= ?orqs |},
+              Hin: In oidx (tl (c_li_indices _)),
+                   Horq: ?orqs@[oidx] = Some _ |- _] =>
+      specialize (Hmcfi oidx _ (in_or_app _ _ _ (or_introl (tl_In _ _ Hin))) Horq);
+      simpl in Hmcfi; destruct Hmcfi
+    | [Hmcf: RsDownConflicts oidx _ ?msgs,
+             Hinm: InMPI ?msgs (?midx, ?msg),
+                   Hmt: msg_type ?msg = MRs |- _] =>
+      specialize (Hmcf (midx, msg) eq_refl
+                       ltac:(simpl; rewrite Hmt; reflexivity)
+                              Hinm); dest; auto
+    end.
+
+Ltac solve_NoRsI_by_rqUp oidx :=
+  repeat
+    match goal with
+    | [Hmcfi: MsgConflictsInv _ _ {| bst_orqs:= ?orqs |},
+              Hin: In oidx (c_li_indices _ ++ c_l1_indices _),
+                   Horq: ?orqs@[oidx] = Some _ |- _] =>
+      specialize (Hmcfi oidx _ Hin Horq);
+      simpl in Hmcfi; destruct Hmcfi
+    | [Hmcf: RsDownConflicts oidx _ ?msgs,
+             Hinm: InMPI ?msgs (?rsd, ?msg),
+                   Hmt: msg_type ?msg = MRs,
+                        Hfmp: FirstMPI ?msgs (?rqu, ?rmsg) |- _] =>
+      specialize (Hmcf (rsd, msg) eq_refl
+                       ltac:(simpl; rewrite Hmt; reflexivity)
+                              Hinm);
+      let Hrqu := fresh "H" in
+      destruct Hmcf as [_ [Hrqu _]];
+      apply Hrqu with (rqUp:= (rqu, rmsg)); auto
+    | |- InMPI _ _ => red; solve_in_mp
+    end.
+
+Ltac solve_NoRsI_by_rqDown oidx :=
+  repeat
+    match goal with
+    | [Hmcfi: MsgConflictsInv _ _ {| bst_orqs:= ?orqs |},
+              Hin: In oidx (c_l1_indices _),
+                   Horq: ?orqs@[oidx] = Some _ |- _] =>
+      specialize (Hmcfi oidx _ (in_or_app _ _ _ (or_intror Hin)) Horq);
+      simpl in Hmcfi; destruct Hmcfi
+    | [Hmcfi: MsgConflictsInv _ _ {| bst_orqs:= ?orqs |},
+              Hin: In oidx (tl (c_li_indices _)),
+                   Horq: ?orqs@[oidx] = Some _ |- _] =>
+      specialize (Hmcfi oidx _ (in_or_app _ _ _ (or_introl (tl_In _ _ Hin))) Horq);
+      simpl in Hmcfi; destruct Hmcfi
+    | [Hmcf: RsDownConflicts oidx _ ?msgs,
+             Hinm: InMPI ?msgs (?midx, ?msg),
+                   Hmt: msg_type ?msg = MRs |- _] =>
+      specialize (Hmcf (midx, msg) eq_refl
+                       ltac:(simpl; rewrite Hmt; reflexivity)
+                              Hinm);
+      let Hrqd := fresh "H" in
+      destruct Hmcf as [_ [_ [_ [Hrqd _]]]];
+      eapply Hrqd; try eassumption; try reflexivity; assumption
+    end.
+
+Ltac solve_NoRsI_by_rsDown oidx :=
+  repeat
+    match goal with
+    | [Hmcfi: MsgConflictsInv _ _ {| bst_orqs:= ?orqs |},
+              Hin: In oidx (c_l1_indices _),
+                   Horq: ?orqs@[oidx] = Some _ |- _] =>
+      specialize (Hmcfi oidx _ (in_or_app _ _ _ (or_intror Hin)) Horq);
+      simpl in Hmcfi; destruct Hmcfi
+    | [Hmcf: RsDownConflicts oidx _ ?msgs,
+             Hinm: InMPI ?msgs (?midx, ?msg),
+                   Hmt: msg_type ?msg = MRs,
+                        Hfmp: FirstMPI ?msgs (?midx, ?rmsg) |- _] =>
+      specialize (Hmcf (midx, msg) eq_refl
+                       ltac:(simpl; rewrite Hmt; reflexivity)
+                              Hinm);
+      let Hrqd := fresh "H" in
+      destruct Hmcf as [_ [_ [Hrqd _]]];
+      eapply Hrqd with (rrsDown:= (midx, rmsg));
+      try eassumption; try reflexivity
+    | |- valOf (_, ?msg1) <> valOf (_, ?msg2) =>
+      let Hx := fresh "H" in
+      destruct msg1, msg2; simpl in *; intro Hx; inv Hx; discriminate
+    | |- InMPI _ _ => red; solve_in_mp
+    end.
+
+Ltac solve_NoRqI_base :=
+  repeat
+    match goal with
+    | |- NoRqI _ _ => do 3 red; intros
+    | |- MsgP _ _ =>
+      red; unfold map, caseDec, fst;
+      repeat (find_if_inside; [simpl|auto])
+    | [H: sigOf ?idm = _ |- _] =>
+      let midx := fresh "midx" in
+      let msg := fresh "msg" in
+      destruct idm as [midx msg]; inv H
+    end.
+
+Ltac solve_NoRqI_by_no_locks oidx :=
+  repeat
+    match goal with
+    | [Hmcfi: MsgConflictsInv _ _ {| bst_orqs:= ?orqs |},
+              Hin: In oidx (c_l1_indices _),
+                   Horq: ?orqs@[oidx] = Some _ |- _] =>
+      specialize (Hmcfi oidx _ (in_or_app _ _ _ (or_intror Hin)) Horq);
+      simpl in Hmcfi; destruct Hmcfi
+    | [Hmcfi: MsgConflictsInv _ _ {| bst_orqs:= ?orqs |},
+              Hin: In oidx (tl (c_li_indices _)),
+                   Horq: ?orqs@[oidx] = Some _ |- _] =>
+      specialize (Hmcfi oidx _ (in_or_app _ _ _ (or_introl (tl_In _ _ Hin))) Horq);
+      simpl in Hmcfi; destruct Hmcfi
+    | [Hmcf: RqUpConflicts oidx _ ?msgs, Hinm: InMPI ?msgs (?midx, ?msg) |- _] =>
+      specialize (Hmcf (midx, msg) eq_refl Hinm); dest; auto
+    end.
+
+Ltac solve_NoRqI_by_rsDown oidx :=
+  repeat
+    match goal with
+    | [Hmcfi: MsgConflictsInv _ _ {| bst_orqs:= ?orqs |},
+              Hin: In oidx (c_l1_indices _),
+                   Horq: ?orqs@[oidx] = Some _ |- _] =>
+      specialize (Hmcfi oidx _ (in_or_app _ _ _ (or_intror Hin)) Horq);
+      simpl in Hmcfi; destruct Hmcfi
+    | [Hmcfi: MsgConflictsInv _ _ {| bst_orqs:= ?orqs |},
+              Hin: In oidx (tl (c_li_indices _)),
+                   Horq: ?orqs@[oidx] = Some _ |- _] =>
+      specialize (Hmcfi oidx _ (in_or_app _ _ _ (or_introl (tl_In _ _ Hin))) Horq);
+      simpl in Hmcfi; destruct Hmcfi
+    | [Hmcf: RsDownConflicts oidx _ ?msgs,
+             Hfmp: FirstMPI ?msgs (?down, ?msg),
+                   Hmt: msg_type ?msg = MRs,
+                        Hinm: InMPI ?msgs (?rqu, ?rmsg) |- _] =>
+      apply FirstMP_InMP in Hfmp;
+      specialize (Hmcf (down, msg) eq_refl
+                       ltac:(simpl; rewrite Hmt; reflexivity)
+                              Hfmp);
+      let Hrqu := fresh "H" in
+      destruct Hmcf as [_ [Hrqu _]];
+      eapply Hrqu with (rqUp:= (rqu, rmsg));
+      try eassumption; try reflexivity
+    end.
+
+Ltac derive_ObjDirE oidx cidx :=
+  match goal with
+  | [Host: ?oss@[oidx] = Some ?ost,
+           Horq: ?orqs@[oidx] = Some ?orq |- _] =>
+    assert (ObjDirE orq ost cidx) by (repeat split; assumption)
+  end.
+
+Ltac derive_ObjDirME oidx cidx :=
+  match goal with
+  | [Host: ?oss@[oidx] = Some ?ost,
+           Horq: ?orqs@[oidx] = Some ?orq |- _] =>
+    assert (ObjDirME orq ost cidx) by (repeat split; assumption)
+  end.
+
+Ltac derive_ObjInvRq oidx :=
+  match goal with
+  | [H: FirstMPI ?msgs (rqUpFrom oidx, ?rmsg) |- _] =>
+    assert (ObjInvRq oidx msgs)
+      by (exists (rqUpFrom oidx, rmsg); split;
+                 [red; simpl; solve_in_mp|unfold sigOf; simpl; congruence])
+  end.
+
+Ltac derive_ObjRqWB_inv oidx :=
+  match goal with
+  | [H: FirstMPI ?msgs (rqUpFrom oidx, ?rmsg) |- _] =>
+    assert (ObjRqWB oidx msgs)
+      by (left; eexists; split;
+          [eapply FirstMP_InMP; eassumption
+          |unfold sigOf; simpl; congruence])
+  end.
+
+Ltac derive_ObjRqWB_push oidx :=
+  match goal with
+  | [H: FirstMPI ?msgs (rqUpFrom oidx, ?rmsg) |- _] =>
+    assert (ObjRqWB oidx msgs)
+      by (right; eexists; split;
+          [eapply FirstMP_InMP; eassumption
+          |unfold sigOf; simpl; congruence])
+  end.
+
+Ltac disc_InvNonWB cidx Hinv :=
+  repeat
+    match goal with
+    | [Hp: parentIdxOf _ cidx = Some _ |- _] =>
+      specialize (Hinv _ _ Hp); simpl in Hinv;
+      disc_rule_conds_ex
+    end.
+
+Ltac disc_InvWBChild cidx Hinv :=
+  match goal with
+  | [Hp: parentIdxOf _ cidx = Some _ |- _] =>
+    specialize (Hinv _ _ Hp); simpl in Hinv;
+    disc_rule_conds_ex
+  end.
+
+Ltac disc_InvWB_inv cidx Hinv :=
+  specialize (Hinv cidx); simpl in Hinv;
+  disc_rule_conds_ex;
+  match goal with
+  | [Hcoh: CohInvRq cidx ?ost _, Ho: ObjOwned ?ost, Hfm: FirstMPI _ _ |- _] =>
+    specialize (Hcoh Ho _ (FirstMP_InMP Hfm));
+    unfold sigOf in Hcoh; simpl in Hcoh;
+    specialize (Hcoh ltac:(congruence))
+  end.
+
+Ltac disc_InvWB_push cidx Hinv :=
+  specialize (Hinv cidx); simpl in Hinv;
+  disc_rule_conds_ex;
+  match goal with
+  | [Hcoh: CohPushRq cidx ?ost _, Ho: ObjOwned ?ost, Hfm: FirstMPI _ _ |- _] =>
+    specialize (Hcoh Ho _ (FirstMP_InMP Hfm));
+    unfold sigOf in Hcoh; simpl in Hcoh;
+    specialize (Hcoh ltac:(congruence))
+  end.
+
+Hint Unfold NoRsI ImplOStateMESI: RuleConds.
 Hint Unfold InvForSim: RuleConds.
 
