src/Ex/InvTemplate.v
@@ -1,0 +1,412 @@
+Require Import List FMap Lia.
+Require Import Common Topology ListSupport IndexSupport.
+Require Import Syntax MessagePool Semantics StepM Invariant.
+Require Import RqRsLang. Import RqRsNotations.
+
+Require Import Ex.TopoTemplate Ex.RuleTemplate.
+
+Set Implicit Arguments.
+
+Local Open Scope list.
+Local Open Scope fmap.
+
+(** Common Invariants that might be shared among various protocols *)
+
+Definition MsgExistsSig (sig: MSig) (msgs: MessagePool Msg) :=
+  exists idm, InMPI msgs idm /\ sigOf idm = sig.
+
+Definition MsgP (spl: list (MSig * (Id Msg -> Prop))) (idm: Id Msg) :=
+  caseDec sig_dec (sigOf idm) True
+          (map (fun sp => (fst sp, snd sp idm)) spl).
+
+Definition MsgsP (spl: list (MSig * (Id Msg -> Prop))) (msgs: MessagePool Msg) :=
+  forall idm, InMPI msgs idm -> MsgP spl idm.
+
+Definition MsgsNotExist (sigs: list MSig) (msgs: MessagePool Msg) :=
+  MsgsP (map (fun sig => (sig, fun _ => False)) sigs) msgs.
+
+Section MsgConflicts.
+
+  Definition RsDownConflicts (oidx: IdxT) (orq: ORq Msg) (msgs: MessagePool Msg) :=
+    forall rsDown,
+      fst (sigOf rsDown) = downTo oidx ->
+      fst (snd (sigOf rsDown)) = MRs ->
+      InMPI msgs rsDown ->
+      (orq@[upRq] <> None) /\
+      (forall rqUp,
+          fst (sigOf rqUp) = rqUpFrom oidx ->
+          InMPI msgs rqUp -> False) /\
+      (forall rrsDown,
+          fst (sigOf rrsDown) = downTo oidx ->
+          fst (snd (sigOf rrsDown)) = MRs ->
+          valOf rsDown <> valOf rrsDown ->
+          InMPI msgs rrsDown -> False) /\
+      (forall rqDown,
+          fst (sigOf rqDown) = downTo oidx ->
+          fst (snd (sigOf rqDown)) = MRq ->
+          FirstMPI msgs rqDown -> False) /\
+      (forall rsUp,
+          fst (sigOf rsUp) = rsUpFrom oidx ->
+          InMPI msgs rsUp -> False).
+
+  Definition RqUpConflicts (oidx: IdxT) (orq: ORq Msg) (msgs: MessagePool Msg) :=
+    forall rqUp,
+      fst (sigOf rqUp) = rqUpFrom oidx ->
+      InMPI msgs rqUp ->
+      (orq@[upRq] <> None) /\
+      (forall rrqUp,
+          fst (sigOf rrqUp) = rqUpFrom oidx ->
+          valOf rqUp <> valOf rrqUp ->
+          InMPI msgs rrqUp -> False) /\
+      (forall rsDown,
+          fst (sigOf rsDown) = downTo oidx ->
+          fst (snd (sigOf rsDown)) = MRs ->
+          InMPI msgs rsDown -> False).
+
+  Variable (tr: tree) (bidx: IdxT).
+  Hypothesis (Htr: tr <> Node nil).
+  Let topo := fst (tree2Topo tr bidx).
+  Let cifc := snd (tree2Topo tr bidx).
+
+  Context `{OStateIfc}.
+  Variable (sys: System).
+  
+  Hypotheses (Hiorqs: GoodORqsInit (initsOf sys))
+             (Hrrs: RqRsSys topo sys)
+             (Hoinds: SubList (c_li_indices cifc ++ c_l1_indices cifc)
+                              (map (@obj_idx _) (sys_objs sys))).
+
+  Definition MsgConflictsInv (st: MState) :=
+    forall oidx orq,
+      In oidx (c_li_indices cifc ++ c_l1_indices cifc) ->
+      (bst_orqs st)@[oidx] = Some orq ->
+      RsDownConflicts oidx orq (bst_msgs st) /\
+      RqUpConflicts oidx orq (bst_msgs st).
+
+  Lemma tree2Topo_MsgConflicts_inv_ok:
+    InvReachable sys step_m MsgConflictsInv.
+  Proof.
+    unfold InvReachable, MsgConflictsInv; intros.
+
+    unfold cifc in H1.
+    rewrite c_li_indices_head_rootOf in H1 by assumption.
+    inv H1.
+
+    1: { (* the root case *)
+      (** TODO: need to prove an invariant about the root (main memory):
+       * no messages exist in any channel of the root, i.e., the RqUp, RsUp,
+       * and Down queues are all empty for the root.
+       *)
+      admit.
+    }
+
+    (* non-root cases *)
+    assert (exists pidx,
+               In pidx (c_li_indices cifc) /\
+               parentIdxOf topo oidx = Some pidx).
+    { apply in_app_or in H3; destruct H3.
+      { apply c_li_indices_tail_has_parent; assumption. }
+      { apply c_l1_indices_has_parent; assumption. }
+    }
+    destruct H1 as [pidx [? ?]].
+
+    pose proof (tree2Topo_TreeTopo tr bidx).
+    destruct H5; dest.
+    specialize (H5 _ _ H4); dest.
+
+    assert (exists obj, In obj (sys_objs sys) /\ obj_idx obj = oidx).
+    { apply in_app_or in H3; destruct H3.
+      { apply tl_In in H3.
+        apply SubList_app_4 in Hoinds; apply Hoinds in H3.
+        apply in_map_iff in H3; destruct H3 as [obj [? ?]]; subst.
+        exists obj; auto.
+      }
+      { apply SubList_app_5 in Hoinds; apply Hoinds in H3.
+        apply in_map_iff in H3; destruct H3 as [obj [? ?]]; subst.
+        exists obj; auto.
+      }
+    }
+    destruct H10 as [obj [? ?]]; subst.
+
+    assert (exists pobj, In pobj (sys_objs sys) /\ obj_idx pobj = pidx).
+    { apply SubList_app_4 in Hoinds; apply Hoinds in H1.
+      apply in_map_iff in H1; destruct H1 as [pobj [? ?]]; subst.
+      exists pobj; auto.
+    }
+    destruct H11 as [pobj [? ?]]; subst.
+
+    split; red; intros; repeat ssplit; intros.
+    - intro Hx.
+      eapply upLocked_rsDown_in_false
+        with (obj0:= obj) (down:= downTo (obj_idx obj))
+             (rsdm:= valOf rsDown); eauto.
+      unfold sigOf in H12; simpl in H12; red in H14; rewrite H12 in H14; assumption.
+    - eapply rqUp_in_rsDown_in_false
+        with (obj0:= obj) (rqUp0:= rqUpFrom (obj_idx obj)) (rqum:= valOf rqUp)
+             (down:= downTo (obj_idx obj)) (rsdm:= valOf rsDown); eauto.
+      + unfold sigOf in H15; simpl in H15; red in H16; rewrite H15 in H16; assumption.
+      + unfold sigOf in H12; simpl in H12; red in H14; rewrite H12 in H14; assumption.
+    - eapply rsDown_in_rsDown_in_false
+        with (obj0:= obj) (down:= downTo (obj_idx obj))
+             (rsdm1:= valOf rsDown) (rsdm2:= valOf rrsDown); eauto.
+      + unfold sigOf in H12; simpl in H12; red in H14; rewrite H12 in H14; assumption.
+      + unfold sigOf in H15; simpl in H15; red in H18; rewrite H15 in H18; assumption.
+    - eapply rsDown_in_rqDown_first_false
+        with (cobj:= obj) (pobj0:= pobj) (down:= downTo (obj_idx obj))
+             (rsdm:= valOf rsDown) (rqdm:= valOf rqDown); eauto.
+      + unfold sigOf in H12; simpl in H12; red in H14; rewrite H12 in H14; assumption.
+      + unfold sigOf in H15; simpl in H15; red in H17; rewrite H15 in H17; assumption.
+    - eapply rsDown_in_rsUp_in_false
+        with (cobj:= obj) (pobj0:= pobj) (rsUp0:= rsUpFrom (obj_idx obj))
+             (down:= downTo (obj_idx obj))
+             (rsdm:= valOf rsDown) (rsum:= valOf rsUp); eauto.
+      + unfold sigOf in H12; simpl in H12; red in H14; rewrite H12 in H14; assumption.
+      + unfold sigOf in H15; simpl in H15; red in H16; rewrite H15 in H16; assumption.
+    - intro Hx.
+      eapply upLocked_rqUp_in_false
+        with (obj0:= obj) (rqUp0:= rqUpFrom (obj_idx obj))
+             (rqum:= valOf rqUp); eauto.
+      unfold sigOf in H12; simpl in H12; red in H13; rewrite H12 in H13; assumption.
+    - eapply rqUp_in_rqUp_in_false
+        with (obj0:= obj) (rqUp0:= rqUpFrom (obj_idx obj))
+             (rqum1:= valOf rqUp) (rqum2:= valOf rrqUp); eauto.
+      + unfold sigOf in H12; simpl in H12; red in H13; rewrite H12 in H13; assumption.
+      + unfold sigOf in H14; simpl in H14; red in H16; rewrite H14 in H16; assumption.
+    - eapply rqUp_in_rsDown_in_false
+        with (obj0:= obj) (rqUp0:= rqUpFrom (obj_idx obj)) (rqum:= valOf rqUp)
+             (down:= downTo (obj_idx obj)) (rsdm:= valOf rsDown); eauto.
+      + unfold sigOf in H12; simpl in H12; red in H13; rewrite H12 in H13; assumption.
+      + unfold sigOf in H14; simpl in H14; red in H16; rewrite H14 in H16; assumption.
+  Admitted.
+
+End MsgConflicts.
+
+Section Facts.
+
+  Lemma MsgsP_enqMP:
+    forall spl msgs,
+      MsgsP spl msgs ->
+      forall midx msg,
+        MsgP spl (midx, msg) ->
+        MsgsP spl (enqMP midx msg msgs).
+  Proof.
+    unfold MsgsP, MsgP; intros.
+    apply InMP_enqMP_or in H1; destruct H1; auto.
+    destruct idm as [midx' msg']; simpl in *; dest; subst.
+    assumption.
+  Qed.
+
+  Lemma MsgsP_other_midx_enqMP:
+    forall spl msgs,
+      MsgsP spl msgs ->
+      forall midx msg,
+        ~ In midx (map (fun sp => fst (fst sp)) spl) ->
+        MsgsP spl (enqMP midx msg msgs).
+  Proof.
+    unfold MsgsP, MsgP; intros.
+    apply InMP_enqMP_or in H1; destruct H1; auto.
+    destruct idm as [midx' msg']; simpl in *; dest; subst.
+    destruct msg as [mid mty mval].
+    unfold sigOf; simpl.
+    clear -H0.
+    induction spl; [simpl; auto|].
+    unfold map; rewrite caseDec_head_neq.
+    - apply IHspl.
+      intro Hx; elim H0; right; assumption.
+    - simpl; intro Hx.
+      elim H0; left.
+      unfold MSig in *; rewrite <-Hx; reflexivity.
+  Qed.
+
+  Lemma MsgsP_other_midx_enqMsgs:
+    forall spl msgs,
+      MsgsP spl msgs ->
+      forall eins,
+        DisjList (idsOf eins) (map (fun sp => fst (fst sp)) spl) ->
+        MsgsP spl (enqMsgs eins msgs).
+  Proof.
+    intros.
+    generalize dependent msgs.
+    induction eins as [|ein eins]; simpl; intros; [assumption|].
+    destruct ein as [midx msg]; simpl in *.
+    apply DisjList_cons in H0; dest.
+    eapply IHeins; eauto.
+    apply MsgsP_other_midx_enqMP; auto.
+  Qed.
+
+  Lemma MsgsP_other_msg_id_enqMP:
+    forall spl msgs,
+      MsgsP spl msgs ->
+      forall midx msg,
+        ~ In (msg_id msg) (map (fun sp => snd (snd (fst sp))) spl) ->
+        MsgsP spl (enqMP midx msg msgs).
+  Proof.
+    unfold MsgsP, MsgP; intros.
+    apply InMP_enqMP_or in H1; destruct H1; auto.
+    destruct idm as [midx' msg']; simpl in *; dest; subst.
+    destruct msg as [mid mty mval]; simpl in H0.
+    unfold sigOf; simpl.
+    clear -H0.
+    induction spl; [simpl; auto|].
+    unfold map; rewrite caseDec_head_neq.
+    - apply IHspl.
+      intro Hx; elim H0; right; assumption.
+    - simpl; intro Hx.
+      elim H0; left.
+      unfold MSig in *; rewrite <-Hx; reflexivity.
+  Qed.
+
+  Lemma MsgsP_other_msg_id_enqMsgs:
+    forall spl msgs,
+      MsgsP spl msgs ->
+      forall eins,
+        DisjList (map (fun idm => msg_id (valOf idm)) eins)
+                 (map (fun sp => snd (snd (fst sp))) spl) ->
+        MsgsP spl (enqMsgs eins msgs).
+  Proof.
+    intros.
+    generalize dependent msgs.
+    induction eins as [|ein eins]; simpl; intros; [assumption|].
+    destruct ein as [midx msg]; simpl in *.
+    apply DisjList_cons in H0; dest.
+    eapply IHeins; eauto.
+    apply MsgsP_other_msg_id_enqMP; auto.
+  Qed.
+
+  Lemma MsgsP_enqMP_inv:
+    forall spl msgs midx msg,
+      MsgsP spl (enqMP midx msg msgs) ->
+      MsgsP spl msgs.
+  Proof.
+    unfold MsgsP; intros.
+    apply H.
+    apply InMP_or_enqMP; auto.
+  Qed.
+
+  Lemma MsgsP_enqMsgs_inv:
+    forall spl msgs eins,
+      MsgsP spl (enqMsgs eins msgs) ->
+      MsgsP spl msgs.
+  Proof.
+    unfold MsgsP; intros.
+    apply H.
+    apply InMP_or_enqMsgs; auto.
+  Qed.
+
+  Lemma MsgsP_deqMP:
+    forall spl msgs,
+      MsgsP spl msgs ->
+      forall midx,
+        MsgsP spl (deqMP midx msgs).
+  Proof.
+    unfold MsgsP; intros.
+    apply InMP_deqMP in H0; auto.
+  Qed.
+
+  Lemma MsgsP_deqMsgs:
+    forall spl msgs,
+      MsgsP spl msgs ->
+      forall minds,
+        MsgsP spl (deqMsgs minds msgs).
+  Proof.
+    unfold MsgsP; intros.
+    apply InMP_deqMsgs in H0; auto.
+  Qed.
+
+  Lemma MsgsP_other_midx_deqMP_inv:
+    forall spl msgs midx,
+      MsgsP spl (deqMP midx msgs) ->
+      ~ In midx (map (fun sp => fst (fst sp)) spl) ->
+      MsgsP spl msgs.
+  Proof.
+    unfold MsgsP, MsgP; intros.
+    destruct (idx_dec midx (idOf idm)); subst;
+      [|apply H; apply deqMP_InMP_midx; auto].
+
+    clear -H0.
+    induction spl; [simpl; auto|].
+    unfold map; rewrite caseDec_head_neq.
+    - apply IHspl.
+      intro Hx; elim H0; right; assumption.
+    - simpl; intro Hx.
+      elim H0; left.
+      unfold MSig in *; rewrite <-Hx; reflexivity.
+  Qed.
+
+  Lemma MsgsP_other_midx_deqMsgs_inv:
+    forall spl minds msgs,
+      MsgsP spl (deqMsgs minds msgs) ->
+      DisjList minds (map (fun sp => fst (fst sp)) spl) ->
+      MsgsP spl msgs.
+  Proof.
+    intros.
+    generalize dependent msgs.
+    induction minds as [|mind minds]; simpl; intros; [assumption|].
+    apply DisjList_cons in H0; dest.
+    eapply MsgsP_other_midx_deqMP_inv.
+    - eapply IHminds; eauto.
+    - assumption.
+  Qed.
+
+  Lemma MsgsP_other_msg_id_deqMP_inv:
+    forall spl msgs midx msg,
+      MsgsP spl (deqMP midx msgs) ->
+      FirstMP msgs midx msg ->
+      ~ In (msg_id msg) (map (fun sp => snd (snd (fst sp))) spl) ->
+      MsgsP spl msgs.
+  Proof.
+    unfold MsgsP, MsgP; intros.
+    destruct (idx_dec midx (idOf idm)); subst;
+      [|apply H; apply deqMP_InMP_midx; auto].
+
+    destruct (msg_dec msg (valOf idm)); subst;
+      [|apply H; eapply deqMP_InMP; eauto; congruence].
+
+    clear -H1.
+    induction spl; [simpl; auto|].
+    unfold map; rewrite caseDec_head_neq.
+    - apply IHspl.
+      intro Hx; elim H1; right; assumption.
+    - simpl; intro Hx.
+      elim H1; left.
+      unfold MSig in *; rewrite <-Hx; reflexivity.
+  Qed.
+
+  Lemma MsgsP_other_msg_id_deqMsgs_inv:
+    forall spl rmsgs msgs,
+      MsgsP spl (deqMsgs (idsOf rmsgs) msgs) ->
+      NoDup (idsOf rmsgs) ->
+      Forall (FirstMPI msgs) rmsgs ->
+      DisjList (map (fun idm => msg_id (valOf idm)) rmsgs)
+               (map (fun sp => snd (snd (fst sp))) spl) ->
+      MsgsP spl msgs.
+  Proof.
+    intros.
+    generalize dependent msgs.
+    induction rmsgs as [|rmsg rmsgs]; simpl; intros; [assumption|].
+    inv H0; inv H1.
+    apply DisjList_cons in H2; dest.
+    eapply MsgsP_other_msg_id_deqMP_inv; eauto.
+    eapply IHrmsgs; eauto.
+    apply FirstMPI_Forall_deqMP; auto.
+  Qed.
+  
+End Facts.
+
+Ltac disc_MsgsP H :=
+  repeat
+    (first [apply MsgsP_enqMsgs_inv in H
+           |apply MsgsP_enqMP_inv in H
+           |apply MsgsP_other_midx_deqMsgs_inv in H; [|solve_DisjList_ex idx_dec]
+           |apply MsgsP_other_midx_deqMP_inv in H; [|solve_chn_not_in; fail]
+           |eapply MsgsP_other_msg_id_deqMP_inv in H;
+            [|eassumption
+             |unfold valOf, snd;
+              match goal with
+              | [Hi: msg_id ?rmsg = _, Hf: FirstMPI _ (_, ?rmsg) |- _] =>
+                rewrite Hi; solve_not_in
+              end]
+    ]).
+
+Hint Unfold MsgsNotExist: RuleConds.
+
