src/Ex/SimTemplate.v
@@ -1,0 +1,352 @@
+Require Import List FMap Lia.
+Require Import Common Topology ListSupport IndexSupport.
+Require Import Syntax MessagePool Semantics StepM Invariant.
+Require Import RqRsLang.
+
+Require Import Ex.TopoTemplate Ex.RuleTemplate Ex.InvTemplate.
+
+Set Implicit Arguments.
+
+Local Open Scope list.
+Local Open Scope fmap.
+
+Import PropMonadNotations.
+
+Section SimExtMP.
+  Variable (l1s: list IdxT).
+
+  Let erqs := map (fun cidx => rqUpFrom (l1ExtOf cidx)) l1s.
+  Let erss := map (fun cidx => downTo (l1ExtOf cidx)) l1s.
+
+  Definition SimExtMP (imsgs: MessagePool Msg) (iorqs: ORqs Msg)
+             (smsgs: MessagePool Msg) :=
+    Forall
+      (fun cidx =>
+         let eidx := l1ExtOf cidx in
+         (corq <-- iorqs@[cidx];
+            (corq@[upRq] >>= (fun rqiu => rqiu.(rqi_msg)))
+              ::> (findQ (rqUpFrom eidx) imsgs) = findQ (rqUpFrom eidx) smsgs) /\
+         findQ (downTo eidx) imsgs = findQ (downTo eidx) smsgs)
+      l1s.
+
+  Ltac disc_SimExtMP :=
+    unfold SimExtMP; intros;
+    repeat
+      match goal with
+      | [ |- Forall _ l1s] =>
+        let cidx := fresh "cidx" in
+        let He := fresh "He" in
+        apply Forall_forall; intros cidx He
+      | [H1: Forall _ l1s, H2: In _ l1s |- _] =>
+        rewrite Forall_forall in H1; specialize (H1 _ H2)
+      end.
+
+  Lemma SimExtMP_enqMsgs:
+    forall eins,
+      NoDup (idsOf eins) ->
+      forall imsgs orqs smsgs,
+        SimExtMP imsgs orqs smsgs ->
+        SimExtMP (enqMsgs eins imsgs) orqs (enqMsgs eins smsgs).
+  Proof.
+    disc_SimExtMP.
+    disc_rule_conds_ex.
+    repeat split.
+    - destruct (in_dec idx_dec (rqUpFrom (l1ExtOf cidx)) (idsOf eins)).
+      + apply in_map_iff in i.
+        destruct i as [[midx msg] ?]; dest; simpl in *; subst.
+        do 2 (erewrite findQ_In_NoDup_enqMsgs; eauto).
+        rewrite ocons_app; congruence.
+      + do 2 (rewrite findQ_not_In_enqMsgs by assumption).
+        assumption.
+    - destruct (in_dec idx_dec (downTo (l1ExtOf cidx)) (idsOf eins)).
+      + apply in_map_iff in i.
+        destruct i as [[midx msg] ?]; dest; simpl in *; subst.
+        do 2 (erewrite findQ_In_NoDup_enqMsgs; eauto).
+        congruence.
+      + do 2 (rewrite findQ_not_In_enqMsgs by assumption).
+        assumption.
+  Qed.
+
+  Corollary SimExtMP_enqMP:
+    forall midx msg imsgs orqs smsgs,
+      SimExtMP imsgs orqs smsgs ->
+      SimExtMP (enqMP midx msg imsgs) orqs (enqMP midx msg smsgs).
+  Proof.
+    intros.
+    eapply SimExtMP_enqMsgs with (eins:= [(midx, msg)]) in H; auto.
+    repeat constructor; intro; dest_in.
+  Qed.
+
+  Lemma SimExtMP_orqs:
+    forall imsgs orqs1 orqs2 smsgs,
+      SimExtMP imsgs orqs1 smsgs ->
+      Forall (fun cidx => orqs1@[cidx] = orqs2@[cidx]) l1s ->
+      SimExtMP imsgs orqs2 smsgs.
+  Proof.
+    disc_SimExtMP.
+    disc_rule_conds_ex.
+  Qed.
+
+  Lemma SimExtMP_ext_outs_deqMsgs:
+    forall eouts,
+      SubList (idsOf eouts) erss ->
+      NoDup (idsOf eouts) ->
+      forall imsgs orqs smsgs,
+        Forall (FirstMPI imsgs) eouts ->
+        SimExtMP imsgs orqs smsgs ->
+        SimExtMP (deqMsgs (idsOf eouts) imsgs) orqs (deqMsgs (idsOf eouts) smsgs).
+  Proof.
+    disc_SimExtMP.
+    disc_rule_conds_ex.
+    repeat split.
+    - destruct (in_dec idx_dec (rqUpFrom (l1ExtOf cidx)) (idsOf eouts)).
+      + exfalso.
+        apply H in i.
+        apply in_map_iff in i; dest.
+        discriminate.
+      + do 2 (rewrite findQ_not_In_deqMsgs by assumption).
+        assumption.
+    - destruct (in_dec idx_dec (downTo (l1ExtOf cidx)) (idsOf eouts)).
+      + apply in_map_iff in i; destruct i as [[midx msg] ?]; dest.
+        simpl in *; subst.
+        apply findQ_deqMsgs_eq; assumption.
+      + do 2 (rewrite findQ_not_In_deqMsgs by assumption).
+        assumption.
+  Qed.
+
+  Lemma SimExtMP_ext_outs_FirstMPI:
+    forall eouts,
+      SubList (idsOf eouts) erss ->
+      NoDup (idsOf eouts) ->
+      forall imsgs orqs smsgs,
+        SimExtMP imsgs orqs smsgs ->
+        Forall (FirstMPI imsgs) eouts ->
+        Forall (FirstMPI smsgs) eouts.
+  Proof.
+    disc_SimExtMP.
+    disc_rule_conds_ex.
+    apply Forall_forall; intros [midx msg] ?.
+    rewrite Forall_forall in H2; specialize (H2 _ H3).
+    apply in_map with (f:= idOf) in H3.
+    apply H in H3; unfold idOf, fst in H3.
+    apply in_map_iff in H3; destruct H3 as [cidx ?]; dest; subst.
+    rewrite Forall_forall in H1; specialize (H1 _ H4); dest.
+    unfold FirstMPI, FirstMP, firstMP in *; simpl in *.
+    congruence.
+  Qed.
+
+  Lemma SimExtMP_outs_deqMP_child:
+    forall cidx msg imsgs (orqs: ORqs Msg) smsgs corq,
+      In cidx l1s ->
+      orqs@[cidx] = Some corq ->
+      corq@[upRq] = None ->
+      FirstMPI imsgs (rqUpFrom (l1ExtOf cidx), msg) ->
+      SimExtMP imsgs orqs smsgs ->
+      SimExtMP (deqMP (rqUpFrom (l1ExtOf cidx)) imsgs) orqs
+               (deqMP (rqUpFrom (l1ExtOf cidx)) smsgs).
+  Proof.
+    disc_SimExtMP.
+    disc_rule_conds_ex.
+    destruct (idx_dec cidx cidx0); subst.
+    - disc_rule_conds_ex.
+      pose proof (findQ_eq_FirstMPI H2 _ H3).
+      apply findQ_In_deqMP_FirstMP in H2.
+      apply findQ_In_deqMP_FirstMP in H5; simpl in *.
+      rewrite <-H2, <-H5 in H3; inv H3.
+      split; auto.
+      do 2 (rewrite findQ_not_In_deqMP by (intro; subst; discriminate)).
+      assumption.
+    - do 2 (rewrite findQ_not_In_deqMP
+             by (intro Hx; injection Hx; intros; auto)).
+      do 2 (rewrite findQ_not_In_deqMP by (intro; subst; discriminate)).
+      split; assumption.
+  Qed.
+  
+  Lemma SimExtMP_impl_enqMP_indep:
+    forall midx msg imsgs (orqs: ORqs Msg) smsgs,
+      ~ In midx (erqs ++ erss) ->
+      SimExtMP imsgs orqs smsgs ->
+      SimExtMP (enqMP midx msg imsgs) orqs smsgs.
+  Proof.
+    disc_SimExtMP.
+    disc_rule_conds_ex.
+    split.
+    - rewrite findQ_not_In_enqMP; [assumption|].
+      intro; subst.
+      elim H; apply in_or_app; left.
+      apply in_map with (f:= fun cidx => rqUpFrom (l1ExtOf cidx)) in He.
+      assumption.
+    - rewrite findQ_not_In_enqMP; [assumption|].
+      intro; subst.
+      elim H. apply in_or_app; right.
+      apply in_map with (f:= fun cidx => downTo (l1ExtOf cidx)) in He.
+      assumption.
+  Qed.
+
+  Lemma SimExtMP_impl_enqMsgs_indep:
+    forall nmsgs imsgs (orqs: ORqs Msg) smsgs,
+      DisjList (idsOf nmsgs) (erqs ++ erss) ->
+      SimExtMP imsgs orqs smsgs ->
+      SimExtMP (enqMsgs nmsgs imsgs) orqs smsgs.
+  Proof.
+    disc_SimExtMP.
+    disc_rule_conds_ex.
+    split.
+    - rewrite findQ_not_In_enqMsgs; [assumption|].
+      eapply DisjList_In_1; [eassumption|].
+      apply in_or_app; left.
+      apply in_map with (f:= fun cidx => rqUpFrom (l1ExtOf cidx)) in He.
+      assumption.
+    - rewrite findQ_not_In_enqMsgs; [assumption|].
+      eapply DisjList_In_1; [eassumption|].
+      apply in_or_app; right.
+      apply in_map with (f:= fun cidx => downTo (l1ExtOf cidx)) in He.
+      assumption.
+  Qed.
+
+  Lemma SimExtMP_impl_deqMP_indep:
+    forall midx imsgs (orqs: ORqs Msg) smsgs,
+      ~ In midx (erqs ++ erss) ->
+      SimExtMP imsgs orqs smsgs ->
+      SimExtMP (deqMP midx imsgs) orqs smsgs.
+  Proof.
+    disc_SimExtMP.
+    disc_rule_conds_ex.
+    split.
+    - rewrite findQ_not_In_deqMP; [assumption|].
+      intro; subst.
+      elim H; apply in_or_app; left.
+      apply in_map with (f:= fun cidx => rqUpFrom (l1ExtOf cidx)) in He.
+      assumption.
+    - rewrite findQ_not_In_deqMP; [assumption|].
+      intro; subst.
+      elim H. apply in_or_app; right.
+      apply in_map with (f:= fun cidx => downTo (l1ExtOf cidx)) in He.
+      assumption.
+  Qed.
+
+  Lemma SimExtMP_impl_deqMsgs_indep:
+    forall minds imsgs (orqs: ORqs Msg) smsgs,
+      DisjList minds (erqs ++ erss) ->
+      SimExtMP imsgs orqs smsgs ->
+      SimExtMP (deqMsgs minds imsgs) orqs smsgs.
+  Proof.
+    disc_SimExtMP.
+    disc_rule_conds_ex.
+    split.
+    - rewrite findQ_not_In_deqMsgs; [assumption|].
+      eapply DisjList_In_1; [eassumption|].
+      apply in_or_app; left.
+      apply in_map with (f:= fun cidx => rqUpFrom (l1ExtOf cidx)) in He.
+      assumption.
+    - rewrite findQ_not_In_deqMsgs; [assumption|].
+      eapply DisjList_In_1; [eassumption|].
+      apply in_or_app; right.
+      apply in_map with (f:= fun cidx => downTo (l1ExtOf cidx)) in He.
+      assumption.
+  Qed.
+
+  Lemma SimExtMP_impl_silent_locked:
+    forall imsgs (orqs: ORqs Msg) smsgs,
+      SimExtMP imsgs orqs smsgs ->
+      forall oidx porq norq,
+        orqs@[oidx] = Some porq -> porq@[upRq] = None ->
+        (norq@[upRq] >>= (fun rqiu => rqiu.(rqi_msg)) = None) ->
+        SimExtMP imsgs (orqs +[oidx <- norq]) smsgs.
+  Proof.
+    disc_SimExtMP.
+    disc_rule_conds_ex.
+    split; assumption.
+  Qed.
+
+  Lemma SimExtMP_impl_silent_unlocked:
+    forall cidx imsgs (orqs: ORqs Msg) smsgs porq rqiu norq,
+      orqs@[cidx] = Some porq ->
+      porq@[upRq] = Some rqiu -> rqiu.(rqi_msg) = None ->
+      norq@[upRq] = None ->
+      SimExtMP imsgs orqs smsgs ->
+      SimExtMP imsgs (orqs +[cidx <- norq]) smsgs.
+  Proof.
+    disc_SimExtMP.
+    disc_rule_conds_ex.
+  Qed.
+
+  Lemma SimExtMP_spec_deqMP_locked:
+    forall cidx imsgs (orqs: ORqs Msg) smsgs porq norq rqiu msg,
+      orqs@[cidx] = Some porq ->
+      porq@[upRq] = None -> norq@[upRq] = Some rqiu ->
+      FirstMPI imsgs (rqUpFrom (l1ExtOf cidx), msg) ->
+      rqiu.(rqi_msg) = Some msg ->
+      SimExtMP imsgs orqs smsgs ->
+      SimExtMP (deqMP (rqUpFrom (l1ExtOf cidx)) imsgs)
+               (orqs +[cidx <- norq]) smsgs.
+  Proof.
+    disc_SimExtMP.
+    disc_rule_conds_ex.
+    - split.
+      + rewrite findQ_In_deqMP_FirstMP; assumption.
+      + rewrite findQ_not_In_deqMP by discriminate; assumption.
+    - split.
+      + rewrite findQ_not_In_deqMP
+          by (intro Hx; subst; injection Hx; intros; auto).
+        assumption.
+      + rewrite findQ_not_In_deqMP by (intro; subst; discriminate).
+        assumption.
+  Qed.
+
+  Lemma SimExtMP_spec_deqMP_unlocked:
+    forall cidx imsgs (orqs: ORqs Msg) smsgs porq rqiu norq,
+      orqs@[cidx] = Some porq ->
+      porq@[upRq] = Some rqiu -> rqiu.(rqi_msg) <> None ->
+      norq@[upRq] = None ->
+      SimExtMP imsgs orqs smsgs ->
+      SimExtMP imsgs (orqs +[cidx <- norq]) (deqMP (rqUpFrom (l1ExtOf cidx)) smsgs).
+  Proof.
+    disc_SimExtMP.
+    disc_rule_conds_ex.
+    - split.
+      + destruct (rqi_msg rqiu); [|exfalso; auto].
+        unfold deqMP, findQ in *; simpl in *.
+        rewrite <-H3; mred.
+      + rewrite findQ_not_In_deqMP by discriminate; assumption.
+    - split.
+      + rewrite findQ_not_In_deqMP
+          by (intro Hx; subst; injection Hx; intros; auto).
+        assumption.
+      + rewrite findQ_not_In_deqMP by (intro; subst; discriminate).
+        assumption.
+  Qed.
+  
+End SimExtMP.
+
+Ltac solve_sim_ext_mp :=
+  repeat
+    (try
+       match goal with
+       | [ |- SimExtMP _ (enqMP _ _ _) _ (enqMP _ _ _) ] =>
+         apply SimExtMP_enqMP
+       | [ |- SimExtMP _ (deqMP ?midx _) _ (deqMP ?midx _) ] =>
+         eapply SimExtMP_outs_deqMP_child; eauto; mred; fail
+       | [ |- SimExtMP _ (enqMP _ _ _) _ _ ] =>
+         apply SimExtMP_impl_enqMP_indep; [solve_not_in_ext_chns; fail|]
+       | [ |- SimExtMP _ (deqMP _ _) _ _ ] =>
+         eapply SimExtMP_spec_deqMP_locked; eauto; [mred|reflexivity]; fail
+       | [ |- SimExtMP _ (deqMP _ _) _ _ ] =>
+         apply SimExtMP_impl_deqMP_indep; [solve_not_in_ext_chns; fail|]
+       | [ |- SimExtMP _ _ _ (deqMP _ _) ] =>
+         eapply SimExtMP_spec_deqMP_unlocked; eauto; [congruence|mred]; fail
+       | [ |- SimExtMP _ (enqMsgs _ _) _ _ ] =>
+         apply SimExtMP_impl_enqMsgs_indep; [solve_ext_chns_disj; fail|]
+       | [ |- SimExtMP _ (deqMsgs _ _) _ _ ] =>
+         apply SimExtMP_impl_deqMsgs_indep; [solve_ext_chns_disj; fail|]
+       | [ |- SimExtMP _ _ (?m +[?k <- ?v]) _ ] =>
+         apply SimExtMP_orqs with (orqs1:= m);
+         [|apply Forall_forall; intros; mred; fail]
+       | [ |- SimExtMP _ _ (_ +[_ <- addRqS _ _ _]) _] =>
+         eapply SimExtMP_impl_silent_locked;
+         [|eassumption|eassumption|unfold addRqS; mred]
+       | [H1: ?porq@[upRq] = Some ?rqi, H2: rqi_msg ?rqi = None
+          |- SimExtMP _ _ (_ +[_ <- ?porq -[upRq]]) _] =>
+         eapply SimExtMP_impl_silent_unlocked; eauto; mred; fail
+       end; try assumption).
+
